Source/DafnyCompilers/CSharp/Compiler.dfy
@@ -1,31 +1,35 @@
 include "../CSharpDafnyAST.dfy"
 include "../CSharpCompat.dfy"
-
-// import opened CSharpSystem
-
-module Utils {
-  function method SeqMap<T, Q>(f: T ~> Q, ts: seq<T>) : seq<Q>
-    reads * // FIXME
-    requires forall t | t in ts :: f.requires(t)
-  {
-    if ts == [] then [] else [f(ts[0])] + SeqMap(f, ts[1..])
-  }
-}
+include "../Library.dfy"
 
 module {:extern "Microsoft.Dafny.Compilers.SelfHosting.CSharp"} CSharpDafnyCompiler {
   import System
   import CSharpDafnyAST
   import opened CSharpUtils
   import opened Microsoft.Dafny
-  import Utils
 
   module AST {
+    import opened Microsoft
+    import C = CSharpDafnyAST
+
+    datatype Tokd<T> =
+      Tokd(tok: Boogie.IToken, val: T)
+
+    // public class LiteralExpr : Expression
+    datatype LiteralExpr =
+      | LitBool(b: bool)
+      | LitInt(i: int)
+      | LitReal(r: real)
+      | LitChar(c: string) // FIXME should this use a char?
+      | LitString(s: string)
+
     datatype Expression =
-      | StringLiteralExpr(str: string)
-      | InvalidExpression
+      | LiteralExpr(lit: LiteralExpr)
+      | InvalidExpr(msg: string)
+      | UnsupportedExpr(expr: C.Expression)
 
     datatype Stmt =
-      | PrintStmt(stmts: seq<Expression>)
+      | PrintStmt(exprs: seq<Expression>)
       | InvalidStmt
 
     type BlockStmt = seq<Stmt>
@@ -36,75 +40,192 @@ module {:extern "Microsoft.Dafny.Compilers.SelfHosting.CSharp"} CSharpDafnyCompi
   }
 
   module Translator {
-    import AST
-    import Utils
+    import opened Lib
     import opened CSharpUtils
-    import CSharpDafnyAST
+    import opened CSharpUtils.System
+    import opened CSharpUtils.Microsoft
+    import C = CSharpDafnyAST
+    import D = AST
 
-    function method TranslateExpression(s: CSharpDafnyAST.Expression) : AST.Expression reads * {
-      if s is CSharpDafnyAST.StringLiteralExpr then
-        var p := s as CSharpDafnyAST.StringLiteralExpr;
-        if p.Value is System.String then
-          AST.StringLiteralExpr(StringUtils.OfCString(p.Value as System.String))
-        else
-          AST.InvalidExpression
-      else AST.InvalidExpression
+    // function method TranslateExpression(c: C.Expression) : D.Expression reads * {
+    //   match c {
+    //   case c: C.LiteralExpr =>
+    //     match c.Value {
+    //     case s: System.String =>
+    //       var str := StringUtils.OfCString(s);
+    //       match c {
+    //       case c: C.CharLiteralExpr =>
+    //         D.LiteralExpr(D.LitChar(str))
+    //       case c: C.StringLiteralExpr =>
+    //         D.LiteralExpr(D.LitString(str))
+    //       case _ =>
+    //         D.InvalidExpr("LiteralExpr with .Value of type string must be a char or a string.")
+    //       }
+    //     case _ => D.UnsupportedExpr(c)
+    //     }
+    //   case _ => D.UnsupportedExpr(c)
+    //   }
+    // }
+
+    // function method TranslateExpression'(c: C.Expression) : D.Expression reads * {
+    //   match c {
+    //   | c: C.LiteralExpr =>
+    //     match c.Value {
+    //     | s: System.String =>
+    //       var str := StringUtils.OfCString(s);
+    //       match c {
+    //       | c: C.CharLiteralExpr =>
+    //         D.LiteralExpr(D.LitChar(str))
+    //       | c: C.StringLiteralExpr =>
+    //         D.LiteralExpr(D.LitString(str))
+    //       | _ =>
+    //         D.InvalidExpr("LiteralExpr with .Value of type string must be a char or a string.")
+    //       }
+    //     | _ => D.UnsupportedExpr(c)
+    //     }
+    //   | _ => D.UnsupportedExpr(c)
+    //   }
+    // }
+
+    function method TranslateExpression(c: C.Expression) : D.Expression reads * {
+      if c is C.LiteralExpr then
+        var l: C.LiteralExpr := c as C.LiteralExpr;
+
+        if l.Value is Bool then
+          D.LiteralExpr(D.LitBool(TypeConv.AsBool(l.Value)))
+        else if l.Value is Numerics.BigInteger then
+          D.LiteralExpr(D.LitInt(TypeConv.AsInt(l.Value)))
+        else if l.Value is BaseTypes.BigDec then
+          D.LiteralExpr(D.LitReal(TypeConv.AsReal(l.Value))) // TODO test
+        else if l.Value is String then
+          var str := TypeConv.AsString(l.Value);
+          if l is C.CharLiteralExpr then
+            D.LiteralExpr(D.LitChar(str))
+          else if l is C.StringLiteralExpr then
+            D.LiteralExpr(D.LitString(str))
+          else
+            D.InvalidExpr("LiteralExpr with .Value of type string must be a char or a string.")
+        else D.UnsupportedExpr(l)
+      else D.UnsupportedExpr(c)
     }
 
-    function method TranslateStatement(s: CSharpDafnyAST.Statement) : AST.Stmt reads * {
-      if s is CSharpDafnyAST.PrintStmt then
-        var p := s as CSharpDafnyAST.PrintStmt;
-        AST.PrintStmt(Utils.SeqMap(TranslateExpression, ListUtils.ToSeq(p.Args)))
-      else AST.InvalidStmt
+    function method TranslateStatement(s: C.Statement) : D.Stmt reads * {
+      if s is C.PrintStmt then
+        var p := s as C.PrintStmt;
+        D.PrintStmt(Seq.Map(TranslateExpression, ListUtils.ToSeq(p.Args)))
+      else D.InvalidStmt
     }
 
-    function method TranslateBlock(b: CSharpDafnyAST.BlockStmt) : AST.BlockStmt reads * {
-      Utils.SeqMap(TranslateStatement, ListUtils.ToSeq(b.Body))
+    function method TranslateBlock(b: C.BlockStmt) : D.BlockStmt reads * {
+      Seq.Map(TranslateStatement, ListUtils.ToSeq(b.Body))
     }
 
-    function method TranslateMethod(m: CSharpDafnyAST.Method) : AST.Method reads * {
-      AST.Method(TranslateBlock(m.methodBody))
+    function method TranslateMethod(m: C.Method) : D.Method reads * {
+      D.Method(TranslateBlock(m.methodBody))
     }
 
-    function method TranslateProgram(p: CSharpDafnyAST.Program) : AST.Program reads * {
-      AST.Program(TranslateMethod(p.MainMethod))
+    function method TranslateProgram(p: C.Program) : D.Program reads * {
+      D.Program(TranslateMethod(p.MainMethod))
+    }
+  }
+
+  module Target {
+    import opened Lib.Datatypes
+
+    datatype StrTree =
+      | Str(s: string)
+      | SepSeq(sep: Option<string>, asts: seq<StrTree>)
+      | Invalid
+
+    function method Seq(asts: seq<StrTree>) : StrTree {
+      SepSeq(None, asts)
+    }
+
+    function method Concat(sep: string, asts: seq<StrTree>) : StrTree {
+      SepSeq(Some(sep), asts)
+    }
+
+    function method Call(fn: string, args: seq<StrTree>) : StrTree {
+      Seq([Str(fn), Str("("), Concat(", ", args), Str(")")])
+    }
+
+    function method SingleQuote(s: StrTree): StrTree {
+      Seq([Str("'"), s, Str("'")])
+    }
+
+    function method DoubleQuote(s: StrTree): StrTree {
+      Seq([Str("\""), s, Str("\"")])
     }
   }
 
   module Compiler {
+    import Lib
     import opened AST
+    import opened Target
+    import opened Lib.Datatypes
+    import opened CSharpUtils
 
-    class CSharpAST {}
+    function method CompileInt(i: int) : StrTree {
+      var istr := Lib.Str.of_int(i, 10);
+      Call("new BigInteger", [Str(istr)])
+    }
 
-    function method CompileExpression(s: Expression) : CSharpAST? {
+    function method CompileExpression(s: Expression) : StrTree {
       match s {
-        case StringLiteralExpr(str) => null
-        case InvalidExpression => null
+        case LiteralExpr(l) =>
+          match l {
+            case LitBool(b: bool) => Str(if b then "true" else "false")
+            case LitInt(i: int) => CompileInt(i)
+            case LitReal(r: real) =>
+              var n, d := TypeConv.Numerator(r), TypeConv.Denominator(r);
+              Call("new BigRational", [CompileInt(n), CompileInt(d)])
+            case LitChar(c: string) => SingleQuote(Str(c))
+            case LitString(s: string) => DoubleQuote(Str(s))
+          }
+        case InvalidExpr => Invalid
       }
     }
 
-    function method CompileStmt(s: Stmt) : CSharpAST? {
+    function method CompilePrint(e: Expression) : StrTree {
+      Seq([Call("DafnyRuntime.Helpers.Print", [CompileExpression(e)]), Str(";")])
+    }
+
+    function method CompileStmt(s: Stmt) : StrTree {
       match s {
-        case PrintStmt(stmts) => null
-        case InvalidStmt => null
+        case PrintStmt(exprs) =>
+          Concat("\n", Lib.Seq.Map(CompilePrint, exprs))
+        case InvalidStmt => Invalid
       }
     }
 
-    function method CompileMethod(m: Method) : CSharpAST? {
+    function method CompileMethod(m: Method) : StrTree {
       match m {
-        case Method(methodBody) => null
+        case Method(methodBody) => Concat("\n", Lib.Seq.Map(CompileStmt, methodBody))
       }
     }
 
-    function method CompileProgram(p: Program) : CSharpAST? {
+    function method CompileProgram(p: Program) : StrTree {
       match p {
         case Program(mainMethod) => CompileMethod(mainMethod)
       }
     }
   }
 
-  method WriteStr(output: ConcreteSyntaxTree, str: string) {
-    output.Write(StringUtils.ToCString(str));
+  method WriteAST(output: ConcreteSyntaxTree, ast: Target.StrTree) {
+    match ast {
+      case Str(s) =>
+        output.Write(StringUtils.ToCString(s));
+      case SepSeq(sep, asts) =>
+        var i := 0;
+        while i < |asts| {
+          if i != 0 && sep.Some? {
+            output.Write(StringUtils.ToCString(sep.t));
+          }
+          WriteAST(output, asts[i]);
+          i := i + 1;
+        }
+      case Invalid =>
+    }
   }
 
   class {:extern} DafnyCSharpCompiler {
@@ -113,7 +234,9 @@ module {:extern "Microsoft.Dafny.Compilers.SelfHosting.CSharp"} CSharpDafnyCompi
 
     method Compile(dafnyProgram: CSharpDafnyAST.Program,
                    output: ConcreteSyntaxTree) {
-      WriteStr(output, "Console.WriteLine(\"Hello, world!\")");
+      var translated := Translator.TranslateProgram(dafnyProgram);
+      var compiled := Compiler.CompileProgram(translated);
+      WriteAST(output, compiled);
     }
 
     method EmitCallToMain(mainMethod: CSharpDafnyAST.Method,
