Source/DafnyCompilers/CSharpCompat.dfy
@@ -10,6 +10,14 @@ module {:extern "System"} {:compile false} System {
     class {:extern} HashSet<T> {}
     class {:extern} Dictionary<TKey, TValue> {}
   }
+
+  module {:extern "System.Numerics"} {:compile false} Numerics {
+    class {:extern} BigInteger {}
+  }
+}
+
+module {:extern "Microsoft.BaseTypes"} {:compile false} Microsoft.BaseTypes {
+  class {:extern} BigDec {}
 }
 
 module {:extern "Microsoft.Dafny"} {:compile false} Microsoft.Dafny {
@@ -38,8 +46,17 @@ module {:extern "Microsoft.Boogie"} {:compile false} Microsoft.Boogie {
   class {:extern} Function {}
 }
 
+module {:extern "DafnyRuntime"} {:compile false} DafnyRuntime {
+  class {:extern} BigRational {
+    var num: int
+    var den: int
+  }
+}
+
 module {:extern "CSharpUtils"} CSharpUtils {
   import System
+  import Microsoft
+  import DafnyRuntime
   import opened System.Collections.Generic
 
   class {:extern} Tuple2<T1, T2> {}
@@ -51,7 +68,7 @@ module {:extern "CSharpUtils"} CSharpUtils {
     static method {:extern} Mk<T>() returns (l: List<T>)
     static method {:extern} Append<T>(l: List<T>, t: T)
 
-    static function method {:extern} ToSeq<T>(l: List<T>) : seq<T> {
+    static function method ToSeq<T>(l: List<T>) : seq<T> {
       FoldR((t, s) => [t] + s, [], l)
     }
 
@@ -67,5 +84,25 @@ module {:extern "CSharpUtils"} CSharpUtils {
   class StringUtils {
     static function method {:extern} ToCString(s: string) : System.String
     static function method {:extern} OfCString(s: System.String) : string
+  }
+
+  class {:extern "bool"} Bool {}
+
+  class TypeConv {
+    static function method {:extern}
+      AsBool(o: Bool) : bool
+    static function method {:extern}
+      AsInt(o: System.Numerics.BigInteger) : int
+    static function method {:extern}
+      AsReal(o: Microsoft.BaseTypes.BigDec) : real
+    // static function method {:extern}
+    //   BigDecNumerator(o: Microsoft.BaseTypes.BigDec) : int
+    // static function method {:extern}
+    //   BigDecDenominator(o: Microsoft.BaseTypes.BigDec) : int
+    static function method {:extern}
+      AsString(o: System.String) : string
+
+    static function method {:extern} Numerator(r: real) : int
+    static function method {:extern} Denominator(r: real) : int
   }
 }
